applicative subtyping lemma written

STLC/stlc.v
@@ -12,10 +12,7 @@ Inductive type : Set :=  (*r type *)
 
 Inductive arg : Set :=
 | arg_empty
-| args (A : type) (S : arg).
-
-Check arg_empty.
-Check (args type_top (args type_int arg_empty)).
+| args (S : arg) (A : type).
 
 Inductive sub : type -> type -> Prop :=    (* defn sub *)
  | sub_Int :
@@ -43,13 +40,81 @@ Inductive appsub : arg -> type -> type -> Prop :=
 | as_Fun : forall (C A B D : type) (S : arg),
     sub C A ->
     appsub S B D ->
-    appsub (args C S) (type_arrow A B) D
+    appsub (args S C) (type_arrow A B) D
 | as_AndL : forall (A B D : type) (S : arg),
     appsub S A D ->
     appsub S (type_and A B) D
 | as_AndR : forall (A B D : type) (S : arg),
     appsub S B D ->
     appsub S (type_and A B) D.
+
+Fixpoint type_stack (S : arg) (A : type) : type :=
+  match S with
+  | arg_empty => A
+  | args S' A' => type_arrow A' (type_stack S' A)
+  end.
+
+Compute (type_stack (args (args (args arg_empty type_int) type_int) type_top)
+                    type_int).
+
+Lemma appsub_coincides_with_sub :
+  forall (S : arg) (A B : type),
+    appsub S A B ->
+    exists (B' : type), B = (type_stack S B').
+Proof.
+  intros S A B H.
+  induction H; eauto.
+  - exists A. unfold type_stack. reflexivity.
+  - inversion IHappsub; subst.
+    exists x. simpl.
+Admitted.
+
+Lemma appsub_reflexivity :
+  forall (S : arg) (A : type),
+    appsub S (type_stack S A) (type_stack S A).
+Proof.
+Admitted.
+
+Fixpoint union_args (S2 S1 : arg) :=
+  match S1 with
+  | arg_empty => S2
+  | args S' A' => union_args (args S2 A') S'
+  end.
+
+(* ., Int, Top, Int *)
+Definition test_union_S2 :=
+  (args (args (args arg_empty type_int) type_top) type_int).
+
+(* ., Top Int, Int *)
+Definition test_union_S1 :=
+  (args (args (args arg_empty type_top) type_int) type_int).
+
+(* ., Int, Top, Int, Top, Int, Int *)
+Compute (union_args test_union_S2 test_union_S1).
+
+Lemma appsub_transitivity :
+  forall (S1 S2 : arg) (A B C : type),
+    appsub S1 A (type_stack S1 B) ->
+    appsub S2 B (type_stack S2 C) ->
+    appsub (union_args S2 S1) A (type_stack S1 (type_stack S2 C)).
+Proof.
+Admitted.
+
+Lemma appsub_to_sub :
+  forall (S : arg) (A B : type),
+  appsub S A B ->
+  sub A B.
+Proof.
+  Admitted.
+
+Lemma sub_to_appsub :
+  forall (S : arg) (A B1 : type),
+    sub A (type_stack S B1) ->
+    exists B2 : type,
+      appsub S A (type_stack S B2) /\ (sub B2 B1).
+Proof.
+  Admitted.
+
 
 Hint Constructors sub : core.
 
